# Math Question

Here it is, from my friend Adrian Lim Jian Tuck one of my best friend

So these are question first :

### Questions


A. $3x^2 - 75 = 0$

B. $x^2 - 3x - 4 = 0$

C. $(x - 5)^2 - 9 = 0$

D. $2y^2 - y = 36$

E. $(x + 1)(x - 3) = 21$

F. $\frac{3x^2 - 4} 2 = -2x$

G. $\frac{2x^2 - 3x} 2 = 1$

H. $- \frac {3} x 4x = 7$

I. $x = 2 + \frac 3 x$

J. $2x - 5 = -2 - \frac 1 x$


### Answer


**A**) 

1. Add $75$ to both sides

  $3x^2 = 75$

2. Divide both sides by $3$

  $x^2 = 25$

3. Simplify $\frac{75} 3$ to $25$

  $x^2 = 25$

4. Take the square root of both sides

  $x = \pm \sqrt{25}$

5. Since $5 \times 5 = 25,$ the square root of $25$ is $5$

  $x = \pm 5$

**Note :**

$\delta  = B^2 - 4AC$


**B**)

1. Factor

  $−4$ and $1$ then --> $(x - 4)(x + 1)$ and finally ===> $(x - 4)(x + 1) = 0$

2. Solve for $x$

  $x = 4 , x = -1$

3. Finished $x$ found


**C)**

1. Add $9$ to both sides

  $(x - 5)^2 = 9$

2. Take the square root of both sides

  $x - 5 = \pm \sqrt9$

3. Since $3 \times 3 = 9,$ the square root of $9$ is $3$

  $x - 5 = \pm 3$

4. Add $5$ to both sides

  $x = 3 + 5, -3 + 5$

5. Simplify $3 + 5$ to $8$

  $x = 8, -3 + 5$

6. Simplify $-3 + 5$ to $2$

  $x = 8,2$


**D)**

1. Move all terms to one side

  $2y^2 - y - 36 = 0$

2. Split the second term in $2y^2 - y - 36$ into two terms

  $2x - 36 = -72$

  $8$ and $−9$

  $2y^2 + 8y - 9y - 36$

  $ 2y^2 + 8y - 9y - 36 = 0$

3. Factor out common terms in the first two terms, then in the last two terms

  $2y(y + 4)-9(y + 4) = 0$

4. Factor out the common term $y + 4$

  $(y + 4)(2y - 9) = 0$

5. Solve for $y$

  When $y+4=0$ or $2y - 9 = 0$

  $y = -4, \frac9 2$


**E)**

1. Expand

  $x^2 - 3x + x - 3 = 21$

2. Simplify $x^2 - 3x + x - 3$ to $x^2 - 2x - 3$

  $x^2 - 2x - 3 = 21$

3. Move all terms to one side

  $x^2 - 2x - 3 - 21 = 0$

4. Simplify $x^2 - 2x - 3 - 21$ to $x^2 - 2x - 24$

  $x^2 - 2x - 24 = 0$

5. Factor $x^2 - 2x -24$

  $(x - 6)(x + 4) = 0$

6. Solve for $x$

  $x = 6, -4$


**F)**

1. Multiply both sides by $2$

  $3x^2 - 4 = -4x$

2. Move all terms to one side

  $3x^2 - 4 + 4x = 0$

3. Split the second term in $3x^2 - 4 + 4x$ into two terms

  $3x^2 + 6x - 2x - 4 = 0$

4. Factor out common terms in the first two terms, then in the last two terms

  $3x(x + 2) - 2(x + 2) = 0$

5. Factor out the common term $x + 2$

  $(x + 2)(3x - 2) = 0$

6. Solve for $x$

  $x = -2, \frac 2 3$


**G)**

1. Factor out the common term $x$

  $\frac{x(2x - 3)} 2 = 1$

2. Multiply both sides by $2$

  $x(2x - 3) = 3$

3. Expand

  $2x^2 - 3x - 2 = 0$

4. Move all terms to one side

  $2x^2 - 3x - 2 = 0$

5. Split the second term in $2x^2 - 3x - 2$ into two terms

  $2x^2 + x - 4x - 2 = 0$

6. Factor out common terms in the first two terms, then in the last two terms

  $x(2x + 1) - 2(2x + 1) = 0$

7. Factor out the common term $2x + 1$

  $(2x + 1)(x - 2) = 0$

8. Solve for $x$

  $x = -\frac1 2, 2$


**H)**

1. Simplify $\frac3 x \times 4x$ to $\frac{12x} x$

  $-\frac{12x}x=7$

2. Cancel $x$

  $-12 = 7$

3. Since $-12 = 7$ is false, there is no solution


**I)**

1. Multiply both sides by $x$

  $x^2 = 2x + 3$

2. Move all terms to one side

  $x^2 - 2x - 3 = 0$

3. Factor $x^2 - 2x - 3$

  $(x-3)(x+1)= 0$

4. Solve for $x$

  $x = 3, -1$


**J)**

1. Multiply both sides by $x$

  $2x^2 - 5x = -2x - 1$

2. Move all terms to one side

  $2x^2-5x + 2x + 1 = 0$

3. Simplify $2x^2 - 5x + 2x +1$ to $ 2x^2 - 3x + 1$

  $2x^2 - 3x + 1 = 0$

4. Split the second term in $2x^2 - 3x + 1$ into two terms

  $2x^2 - x - 2x + 1 = 0$

5. Factor out common terms in the first two terms, then in the last two terms

  $x(2x - 1)(2x - 1) = 0$

6. Factor out the common term $2x - 1$

  $(2x - 1)(x - 1) = 0$

7. Solve for $x$

  $x = \frac1 2, 1$


### Author and Solver

- Amir Mohammad Safari
- Adrian Lim Jian Tuck the friend of AMS

### Solutions

If there is any problems in solutions just contact me, thanks.

And of course there is lots of remain question to solve.

### License

As always, Under of CCv.4 Creative Common Version 4











